SP1Foundations/MemoryConsistency.lean
@@ -1,9 +1,11 @@
 import SP1Foundations.Word
 
+@[ext]
 structure MemoryAccessInShardTimestamp (F : Type) where
   prev_low : F
   diff_low_limb : F
 
+@[ext]
 structure MemoryAccessInSharedCols (F : Type) where
   prev_value : Word F
   access_timestamp : MemoryAccessInShardTimestamp F
